WIP

src/Closing.v
@@ -1,7 +1,7 @@
 Require Import String PeanoNat Compare_dec StrictProp.
 Require Import Morph Var.
 
-Definition raw_closing := list push_op.
+Definition raw_closing := list (option var).
 
 Definition is_raw_closing_nil (r : raw_closing) :=
   match r with
@@ -12,17 +12,17 @@ Definition is_raw_closing_nil (r : raw_closing) :=
 Fixpoint normalized_raw_closing r :=
   match r with
   | nil => sUnit
-  | cons op r =>
-    if andb (is_zero_push_op op) (is_raw_closing_nil r) then
-      sEmpty
-    else
-      normalized_raw_closing r
+  | cons vo r =>
+    if andb (var_opt_eqb vo zero_var_opt)
+            (is_raw_closing_nil r)
+    then sEmpty
+    else normalized_raw_closing r
   end.
 
-Definition normalized_raw_closing_from_cons {r op} :
-  normalized_raw_closing (cons op r) ->
+Definition normalized_raw_closing_from_cons {r vo} :
+  normalized_raw_closing (cons vo r) ->
   normalized_raw_closing r.
-Proof. destruct op as [|[]|], r; easy. Qed.
+Proof. destruct vo as [[|[]]|], r; easy. Defined.
 
 Set Primitive Projections.
 Record closing :=
@@ -36,54 +36,58 @@ Unset Primitive Projections.
 Definition closing_id : closing :=
   mkclosing nil stt.
 
-Definition normalized_raw_closing_push0 r op :=
-  if andb (is_zero_push_op op) (is_raw_closing_nil r) then nil
-  else cons op r.
+Definition normalized_raw_closing_push0 r vo :=
+  if andb (var_opt_eqb vo zero_var_opt)
+          (is_raw_closing_nil r)
+  then nil
+  else cons vo r.
 
-Definition normalized_raw_closing_push0_normalized
-           {r op} :
+Definition normalized_raw_closing_push0_normalized {r vo} :
   normalized_raw_closing r ->
-  normalized_raw_closing (normalized_raw_closing_push0 r op).
-Proof. intros; destruct op as [|[]|], r; easy. Defined.
+  normalized_raw_closing (normalized_raw_closing_push0 r vo).
+Proof. destruct vo as [[|[]]|], r; easy. Defined.
 
-Definition closing_push0 r op :=
+Definition closing_push0 r vo :=
   mkclosing
-    (normalized_raw_closing_push0 (c_raw r) op)
+    (normalized_raw_closing_push0 (c_raw r) vo)
     (normalized_raw_closing_push0_normalized
        (c_normalized r)).
 
-Definition closing_weak0 r := closing_push0 r weak_op.
+Definition closing_weak0 r :=
+  closing_push0 r None.
 
 Definition closing_exchange0 r l :=
-  closing_push0 r (cycle_in_op l).
+  closing_push0 r (Some (bound l)).
 
-Definition closing_close0 r n := closing_push0 r (close_op n).
+Definition closing_close0 r n :=
+  closing_push0 r (Some (free n)).
 
-Fixpoint closing_push l r op :=
+Fixpoint closing_push l r vo :=
   match l with
-  | 0 => closing_push0 r op
+  | 0 => closing_push0 r vo
   | S l =>
     match r with
     | mkclosing nil norm =>
       closing_push0
-        (closing_push l r (unshift_push zero_push_op op))
-        (shift_push op zero_push_op)
-    | mkclosing (cons op' r) norm =>
+        (closing_push l r (unshift_var_opt zero_var_opt vo))
+        (shift_var_opt vo zero_var_opt)
+    | mkclosing (cons vo' r) norm =>
       closing_push0
         (closing_push l
            (mkclosing r (normalized_raw_closing_from_cons norm))
-           (unshift_push op' op))
-        (shift_push op op')
+           (unshift_var_opt vo' vo))
+        (shift_var_opt vo vo')
     end
   end.
 
-Definition closing_weak l r := closing_push l r weak_op.
+Definition closing_weak l r :=
+  closing_push l r None.
 
 Definition closing_exchange l1 r l2 :=
-  closing_push l1 r (cycle_in_op l2).
+  closing_push l1 r (Some (bound l2)).
 
 Definition closing_close l r n :=
-  closing_push l r (close_op n).
+  closing_push l r (Some (free n)).
 
 Fixpoint closing_weak_n N : closing :=
   match N with
@@ -100,8 +104,8 @@ Fixpoint closing_weakening N M : closing :=
 Fixpoint apply_raw_closing_var r : var_op :=
   match r with
   | nil => var_op_id
-  | cons op r =>
-    lift_var_op (apply_raw_closing_var r) @ apply_push_op_var op
+  | cons vo r =>
+    lift_var_op (apply_raw_closing_var r) @ push_var vo
   end.
 
 Definition apply_closing_var r :=
@@ -111,7 +115,7 @@ Set Primitive Projections.
 Record closing_rhs :=
   mk_closing_rhs {
       rhs_raw_closing : raw_closing;
-      rhs_push : push_op
+      rhs_push : option var
     }.
 Add Printing Constructor closing_rhs.
 Unset Primitive Projections.
@@ -119,60 +123,60 @@ Unset Primitive Projections.
 Definition normalized_closing_rhs r :=
   normalized_raw_closing (rhs_raw_closing r).
 
-Definition closing_rhs_push0 r op :=
+Definition closing_rhs_push0 r vo :=
   mk_closing_rhs
     (normalized_raw_closing_push0 (rhs_raw_closing r)
-       (unshift_push (rhs_push r) op))
-    (shift_push op (rhs_push r)).
+       (unshift_var_opt (rhs_push r) vo))
+    (shift_var_opt vo (rhs_push r)).
 
 Definition closing_rhs_weak0 r :=
-  closing_rhs_push0 r weak_op.
+  closing_rhs_push0 r None.
 
 Definition closing_rhs_exchange0 r l :=
-  closing_rhs_push0 r (cycle_in_op l).
+  closing_rhs_push0 r (Some (bound l)).
 
 Definition closing_rhs_close0 r n :=
-  closing_rhs_push0 r (close_op n).
+  closing_rhs_push0 r (Some (free n)).
 
-Definition closing_rhs_push0_normalized {r op} :
+Definition closing_rhs_push0_normalized {r vo} :
   normalized_closing_rhs r ->
   normalized_closing_rhs
-    (closing_rhs_push0 r op).
+    (closing_rhs_push0 r vo).
 Proof.
   destruct r as [? []]; cbn;
     apply normalized_raw_closing_push0_normalized;
     easy.
 Defined.
 
-Fixpoint transpose_push_raw_closing op r {struct r} :=
+Fixpoint transpose_push_raw_closing vo r {struct r} :=
   match r with
-  | nil => mk_closing_rhs nil op
-  | cons op' r =>
-    if is_zero_push_op op then mk_closing_rhs r op'
+  | nil => mk_closing_rhs nil vo
+  | cons vo' r =>
+    if var_opt_eqb vo zero_var_opt then mk_closing_rhs r vo'
     else closing_rhs_push0
            (transpose_push_raw_closing
-              (unshift_push zero_push_op op) r)
-           op'
+              (unshift_var_var_opt zero_var vo) r)
+           vo'
   end.
 
-Definition transpose_push_raw_closing_normalized {op r} :
+Definition transpose_push_raw_closing_normalized {vo r} :
   normalized_raw_closing r ->
   normalized_closing_rhs
-    (transpose_push_raw_closing op r).
+    (transpose_push_raw_closing vo r).
 Proof.
-  generalize dependent op.
-  induction r as [|op' r]; intros op norm; try easy; cbn.
+  generalize dependent vo.
+  induction r as [|vo' r]; intros vo norm; try easy; cbn.
   apply normalized_raw_closing_from_cons in norm.
-  destruct (is_zero_push_op op); try easy.
+  destruct (var_opt_eqb vo zero_var_opt); try easy.
   apply closing_rhs_push0_normalized.
   apply IHr; easy.
-Qed.
+Defined.
 
 Fixpoint compose_raw_closing r1 r2 :=
   match r1 with
   | nil => r2
-  | cons op r1 =>
-    let rhs := transpose_push_raw_closing op r2 in
+  | cons vo r1 =>
+    let rhs := transpose_push_raw_closing vo r2 in
     normalized_raw_closing_push0
       (compose_raw_closing r1 (rhs_raw_closing rhs))
       (rhs_push rhs)
@@ -184,12 +188,12 @@ Definition compose_raw_closing_normalized {r1 r2} :
   normalized_raw_closing (compose_raw_closing r1 r2).
 Proof.
   generalize dependent r2.
-  induction r1 as [|op]; intros r2 norm1 norm2; try easy.
+  induction r1 as [|vo]; intros r2 norm1 norm2; try easy.
   apply normalized_raw_closing_from_cons in norm1; cbn.
   apply normalized_raw_closing_push0_normalized.
   apply IHr1; try easy.
   apply transpose_push_raw_closing_normalized; easy.
-Qed.
+Defined.
 
 Definition compose_closing r1 r2 :=
   mkclosing
