src/ClosingEquations.v
@@ -14,66 +14,136 @@ Definition lift_closing_eq {c1 c2} :
     end.
 Arguments lift_closing_eq {c1 c2} Heq {n1 n2}.
 
-Lemma apply_normalized_raw_closing_push0 r op :
-  apply_raw_closing_var
-    (normalized_raw_closing_push0 r op)
-  =v= apply_raw_closing_var (cons op r).
+(* Tactic for simplifying comparisons with [zero_var_opt] *)
+
+Lemma reduce_var_opt_eqb_zero_neq vo :
+  vo <> zero_var_opt ->
+  var_opt_eqb vo zero_var_opt = false.
 Proof.
-  destruct op as [|[]|], r; try easy; cbn; simplify_var_ops.
-  rewrite cycle_in_zero_identity; easy.
+  intros; unfold var_opt_eqb.
+  destruct (var_opt_dec vo zero_var_opt); easy.
 Qed.
 
-Lemma normalized_raw_closing_push0_identity r op :
-  normalized_raw_closing (cons op r) ->
-  cons op r = normalized_raw_closing_push0 r op.
-Proof. destruct op as [|[]|], r; easy. Qed.
+Lemma reduce_var_opt_eqb_zero_shift vo1 vo2 :
+  var_opt_eqb (shift_var_opt vo1 vo2) zero_var_opt
+  = andb
+      (var_opt_eqb vo2 zero_var_opt)
+      (negb (var_opt_eqb vo1 zero_var_opt)).
+Proof.
+  destruct vo1 as [v1|], vo2 as [v2|]; cbn; try easy.
+  - case_var v1 as n1 l1; case_var v2 as n2 l2; cbn; try easy.
+    + rewrite Bool.andb_true_r; easy.
+    + case_levels l1 l2.
+      * case_level l2; easy.
+      * rewrite Bool.andb_negb_r; easy.
+      * case_level l1.
+        rewrite Bool.andb_true_r; easy.
+  - rewrite Bool.andb_true_r; easy.
+Qed.
+
+Lemma reduce_var_opt_eqb_zero_unshift vo1 vo2 :
+  vo1 <> zero_var_opt ->
+  vo2 <> zero_var_opt ->
+  var_opt_eqb (unshift_var_opt vo1 vo2) zero_var_opt = false.
+Proof.
+  intros.
+  destruct vo1 as [v1|], vo2 as [v2|]; cbn; try easy.
+  - case_var v1 as n1 l1; case_var v2 as n2 l2;
+      cbn; try easy.
+    + apply reduce_var_opt_eqb_zero_neq; easy.
+    + case_levels l1 l2;
+        try apply reduce_var_opt_eqb_zero_neq; try easy.
+      case_level l2 as l2.
+      case_level l2; try easy.
+      case_level l1; easy.
+  - case_var v2 as n2 v2; try easy.
+    apply reduce_var_opt_eqb_zero_neq; easy.
+Qed.
+
+Hint Rewrite reduce_var_opt_eqb_zero_shift
+     Bool.andb_true_r Bool.andb_false_r : reduce_var_zero.
+
+Hint Rewrite reduce_var_opt_eqb_zero_neq
+     reduce_var_opt_eqb_zero_unshift
+     using (cbn; congruence) : reduce_var_zero.
+
+Ltac reduce_var_zero :=
+  try repeat
+      (autorewrite with reduce_var_zero; cbn in *);
+  try repeat
+    ((rewrite_strat (bottomup (hints reduce_var_zero))); cbn in *).
+
+Ltac case_var_zero vo :=
+  destruct (var_opt_dec vo zero_var_opt);
+    [replace vo with zero_var_opt by easy|];
+    reduce_var_zero.
+
+Lemma apply_normalized_raw_closing_push0 r vo :
+  apply_raw_closing_var
+    (normalized_raw_closing_push0 r vo)
+  =v= apply_raw_closing_var (cons vo r).
+Proof.
+  unfold normalized_raw_closing_push0; cbn.
+  case_var_zero vo; destruct r; cbn; try easy.
+  simplify_var_ops.
+  rewrite push_zero_identity; easy.
+Qed.
+
+Lemma normalized_raw_closing_push0_identity r vo :
+  normalized_raw_closing (cons vo r) ->
+  cons vo r = normalized_raw_closing_push0 r vo.
+Proof.
+  unfold normalized_raw_closing_push0.
+  case_var_zero vo; destruct r; easy.
+Qed.
 
 Definition apply_closing_rhs_var r : var_op :=
   lift_var_op (apply_raw_closing_var (rhs_raw_closing r))
-  @ apply_push_op_var (rhs_push r).
+  @ push_var (rhs_push r).
 
-Lemma apply_closing_rhs_push0 r op :
-  apply_closing_rhs_var (closing_rhs_push0 r op)
+Lemma apply_closing_rhs_push0 r vo :
+  apply_closing_rhs_var (closing_rhs_push0 r vo)
   =v= swap_var
       @ lift_var_op (apply_closing_rhs_var r)
-      @ apply_push_op_var op.
+      @ push_var vo.
 Proof.
   unfold apply_closing_rhs_var; cbn.
-  rewrite apply_normalized_raw_closing_push0; cbn; simplify_var_ops.
+  rewrite apply_normalized_raw_closing_push0;
+    cbn; simplify_var_ops.
   rewrite transpose_swap_lifted'.
-  rewrite transpose_pushes with (op1 := rhs_push r).
+  rewrite transpose_pushes with (vo1 := rhs_push r).
   rewrite swap_swap_identity'.
   easy.
 Qed.
 
 Lemma apply_raw_closing_var_add_cycle_out r :
   apply_raw_closing_var r
-  =v= apply_pop_op_var (cycle_out_op 0) @ apply_raw_closing_var r.
+  =v= pop_var zero_var @ apply_raw_closing_var r.
 Proof.
-  rewrite cycle_out_zero_identity; simplify_var_ops; easy.
+  rewrite pop_zero_identity; simplify_var_ops; easy.
 Qed.
 
-Lemma apply_transpose_push_raw_closing op r :
-  apply_push_op_var op @ apply_raw_closing_var r
+Lemma apply_transpose_push_raw_closing vo r :
+  push_var vo @ apply_raw_closing_var r
   =v=
-  apply_closing_rhs_var (transpose_push_raw_closing op r).
+  apply_closing_rhs_var (transpose_push_raw_closing vo r).
 Proof.
-  generalize dependent op.
-  induction r; intro l';
+  generalize dependent vo.
+  induction r; intro vo';
     rewrite apply_raw_closing_var_add_cycle_out;
     cbn; simplify_var_ops.
   - unfold apply_closing_rhs_var; cbn; simplify_var_ops.
-    rewrite cycle_out_zero_identity; easy.
-  - destruct (is_zero_push_op l') eqn:Heq.
-    + destruct l' as [|[]|]; try easy; cbn.
-      rewrite cycle_in_cycle_out_identity'; easy.
+    rewrite pop_zero_identity; easy.
+  - case_var_zero vo'.
+    + rewrite push_pop_identity' with (v := zero_var); easy.
     + rewrite var_op_associative.
-      fold (apply_pop_op_var (cycle_out_op 0)).
-      rewrite transpose_push_pop by (destruct l' as [|[]|]; easy).
+      fold (pop_var (bound 0)).
+      rewrite transpose_push_pop by easy.
       rewrite apply_closing_rhs_push0; cbn.
       rewrite <- IHr; cbn.
-      destruct l' as [|[]|]; cbn;
-        rewrite cycle_out_zero_identity; simplify_var_ops; easy.
+      rewrite transpose_push_pop_zero_left.
+      rewrite pop_zero_identity.
+      simplify_var_ops; easy.
 Qed.
 
 Lemma apply_compose_raw_closing r1 r2 :
@@ -81,7 +151,7 @@ Lemma apply_compose_raw_closing r1 r2 :
   =v= apply_raw_closing_var r1 @ apply_raw_closing_var r2.
 Proof.
   generalize dependent r2.
-  induction r1 as [|op r1]; intro r2; cbn; try easy.
+  induction r1 as [|vo r1]; intro r2; cbn; try easy.
   simplify_var_ops.
   rewrite apply_normalized_raw_closing_push0; cbn.
   rewrite apply_transpose_push_raw_closing, IHr1.
@@ -107,11 +177,12 @@ Lemma raw_closing_right_identity r :
   normalized_raw_closing r ->
   compose_raw_closing r nil = r.
 Proof.
-  induction r as [|op r]; intros Hnorm; cbn; try easy.
-  - rewrite normalized_raw_closing_push0_identity
-      by easy.
-    rewrite IHr; cbn in *; try easy.
-    destruct op as [|[]|], r; easy.
+  induction r as [|vo r]; intros Hnorm; cbn; try easy.
+  rewrite normalized_raw_closing_push0_identity
+    by easy.
+  rewrite IHr; cbn in *; try easy.
+  generalize Hnorm.
+  case_var_zero vo; destruct r; easy.
 Qed.
 
 Lemma closing_right_identity r :
@@ -122,401 +193,278 @@ Proof.
   apply raw_closing_right_identity; easy.
 Qed.
 
-Fixpoint transpose_push_raw_closing_push op r {struct r} :=
+Fixpoint transpose_push_raw_closing_push vo r {struct r} :=
   match r with
-  | raw_closing_id => op
-  | raw_closing_weak0 r =>
-    match op with
-    | weak_op =>
-      transpose_push_raw_closing_push weak_op r
-    | cycle_in_op 0 => weak_op
-    | cycle_in_op (S l') =>
-      transpose_push_raw_closing_push (cycle_in_op l') r
-    | close_op n =>
-      transpose_push_raw_closing_push (close_op n) r
-    end
-  | raw_closing_exchange0 r l2 =>
-    shift_level_push l2
-      (match op with
-       | weak_op =>
-         transpose_push_raw_closing_push weak_op r
-       | cycle_in_op 0 => cycle_in_op l2
-       | cycle_in_op (S l') =>
-         transpose_push_raw_closing_push (cycle_in_op l') r
-       | close_op n =>
-         transpose_push_raw_closing_push (close_op n) r)
-    end
-
-
-    match l with
-    | 0 => cycle_in_op l2
-    | S l' =>
-      shift_level_push l2
-        (transpose_level_raw_closing_push l' r)
-    end
-  | raw_closing_close0 r n =>
-    match l with
-    | 0 => close_op n
-    | S l' =>
-      shift_name_push n
-        (transpose_level_raw_closing_push l' r)
-    end
+  | nil => vo
+  | cons vo' r =>
+    if var_opt_eqb vo zero_var_opt then vo'
+    else shift_var_opt vo'
+           (transpose_push_raw_closing_push
+              (unshift_var_var_opt zero_var vo) r)
   end.
 
-Lemma rhs_push_transpose_level_raw_closing l r :
-  rhs_push (transpose_level_raw_closing l r)
-  = transpose_level_raw_closing_push l r.
+Lemma rhs_push_transpose_push_raw_closing vo r :
+  rhs_push (transpose_push_raw_closing vo r)
+  = transpose_push_raw_closing_push vo r.
 Proof.
-  generalize dependent l.
-  induction r; try easy; intros l'; destruct l';
-    cbn; try easy.
-  - rewrite <- IHr.
-    destruct (transpose_level_raw_closing l' r) as [? []];
-      easy.
-  - rewrite <- IHr.
-    destruct (transpose_level_raw_closing l' r) as [? []];
-      easy.
+  generalize dependent vo.
+  induction r as [|vo' r]; intros vo; cbn; try easy.
+  case_var_zero vo; try easy.
+  rewrite IHr; easy.
 Qed.
 
-Fixpoint transpose_name_raw_closing_push n r :=
+Fixpoint transpose_push_raw_closing_raw_closing
+         vo r {struct r} :=
   match r with
-  | raw_closing_id => (close_op n)
-  | raw_closing_weak0 r =>
-    transpose_name_raw_closing_push n r
-  | raw_closing_exchange0 r l =>
-    shift_level_push l
-      (transpose_name_raw_closing_push n r)
-  | raw_closing_close0 r n2 =>
-    shift_name_push n2
-      (transpose_name_raw_closing_push n r)
+  | nil => nil
+  | cons vo' r =>
+    if var_opt_eqb vo zero_var_opt then r
+    else
+      normalized_raw_closing_push0
+        (transpose_push_raw_closing_raw_closing
+           (unshift_var_var_opt zero_var vo) r)
+        (unshift_var_opt
+           (transpose_push_raw_closing_push
+              (unshift_var_var_opt zero_var vo) r)
+           vo')
   end.
 
-Lemma rhs_push_transpose_name_raw_closing n r :
-  rhs_push (transpose_name_raw_closing n r)
-  = transpose_name_raw_closing_push n r.
+Lemma rhs_raw_closing_transpose_push_raw_closing vo r :
+  rhs_raw_closing (transpose_push_raw_closing vo r)
+  = transpose_push_raw_closing_raw_closing vo r.
 Proof.
-  induction r; cbn; try easy.
-  - rewrite <- IHr.
-    destruct (transpose_name_raw_closing n r) as [? []];
+  generalize dependent vo.
+  induction r as [|vo' r]; intros vo; cbn; try easy.
+  case_var_zero vo; try easy.
+  rewrite rhs_push_transpose_push_raw_closing, IHr; easy.
+Qed.
+
+Lemma closing_rhs_eta r :
+  r = mk_closing_rhs (rhs_raw_closing r) (rhs_push r).
+Proof. easy. Qed.
+
+Lemma transpose_push_raw_closing_eta vo r :
+  transpose_push_raw_closing vo r
+  = mk_closing_rhs
+      (transpose_push_raw_closing_raw_closing vo r)
+      (transpose_push_raw_closing_push vo r).
+Proof.
+  rewrite closing_rhs_eta
+    with (r := transpose_push_raw_closing vo r).
+  rewrite rhs_raw_closing_transpose_push_raw_closing.
+  rewrite rhs_push_transpose_push_raw_closing.
+  easy.
+Qed.
+
+Lemma transpose_push_raw_closing_raw_closing_normalized vo r :
+  normalized_raw_closing r ->
+  normalized_raw_closing
+    (transpose_push_raw_closing_raw_closing vo r).
+Proof.
+  rewrite <- rhs_raw_closing_transpose_push_raw_closing.
+  apply transpose_push_raw_closing_normalized; easy.
+Qed.
+
+Lemma transpose_push_normalized_raw_closing_push0_push
+      vo1 r vo2 :
+  transpose_push_raw_closing_push vo1
+    (normalized_raw_closing_push0 r vo2)
+  = transpose_push_raw_closing_push vo1 (cons vo2 r).
+Proof.
+  unfold normalized_raw_closing_push0.
+  case_var_zero vo2; destruct r; cbn;
+    case_var_zero vo1; try easy.
+  rewrite transpose_push_reducing_pop_push; try easy.
+  unfold zero_var_opt, zero_var in *; congruence.
+Qed.
+
+Lemma transpose_push_normalized_raw_closing_push0_raw_closing
+      vo1 r vo2 :
+  transpose_push_raw_closing_raw_closing vo1
+    (normalized_raw_closing_push0 r vo2)
+  = transpose_push_raw_closing_raw_closing vo1 (cons vo2 r).
+Proof.
+  unfold normalized_raw_closing_push0.
+  case_var_zero vo2; destruct r; cbn;
+    case_var_zero vo1; try easy.
+  rewrite transpose_push_push_zero_left; easy.
+Qed.
+
+Lemma compose_normalized_raw_closing_push0 r1 vo r2 :
+  normalized_raw_closing r2 ->
+  compose_raw_closing
+    (normalized_raw_closing_push0 r1 vo) r2
+  = compose_raw_closing (cons vo r1) r2.
+Proof.
+  unfold normalized_raw_closing_push0.
+  case_var_zero vo; destruct r1; cbn; try easy.
+  induction r2 as [|vo' r2]; cbn in *; try easy.
+  unfold normalized_raw_closing_push0.
+  case_var_zero vo'; destruct r2; cbn; easy.
+Qed.
+
+Lemma transpose_push_raw_closing_reverse_right vo1 vo2 r :
+  shift_var_opt (transpose_push_raw_closing_push vo1 r)
+    (transpose_push_raw_closing_push vo2
+       (transpose_push_raw_closing_raw_closing vo1 r)) =
+  transpose_push_raw_closing_push (shift_var_opt vo1 vo2) r.
+Proof.
+  generalize dependent vo1.
+  generalize dependent vo2.
+  induction r as [|vo3 r]; intros vo2 vo1; cbn; try easy.
+  case_var_zero vo1.
+  - rewrite transpose_push_reducing_push_pop; easy.
+  - rewrite transpose_push_normalized_raw_closing_push0_push; cbn.
+    case_var_zero vo2.
+    + apply transpose_pushes_squared_right.
+    + rewrite transpose_pushes_reverse_right.
+      rewrite IHr.
+      rewrite transpose_push_push_pop_zero_reverse_right
+        by easy.
       easy.
-  - rewrite <- IHr.
-    destruct (transpose_name_raw_closing n r) as [? []];
-      easy.
 Qed.
 
-Definition transpose_push_raw_closing_push p r :=
-  match p with
-  | weak_op => weak_op
-  | cycle_in_op l => transpose_level_raw_closing_push l r
-  | close_op n => transpose_name_raw_closing_push n r
-  end.
-
-Lemma transpose_level_push_normalized_raw_closing_exchange0
-      l1 r l2 :
-  transpose_level_raw_closing_push l1
-    (normalized_raw_closing_exchange0 r l2)
-  = transpose_level_raw_closing_push l1
-      (raw_closing_exchange0 r l2).
-Proof.
-  destruct l2, r; cbn; try easy.
-  destruct l1; easy.
-Qed.
-
-Lemma transpose_name_push_normalized_raw_closing_exchange0
-      n r l :
-  transpose_name_raw_closing_push n
-    (normalized_raw_closing_exchange0 r l)
-  = transpose_name_raw_closing_push n
-      (raw_closing_exchange0 r l).
-Proof. destruct l, r; easy. Qed.
-
-Lemma transpose_level_push_compose_exchange0 l1 l2 r1 r2 :
-  transpose_level_raw_closing_push (S l1)
-    (compose_raw_closing (raw_closing_exchange0 r1 l2) r2)
-= shift_push (transpose_level_raw_closing_push l2 r2)
-    (transpose_level_raw_closing_push l1
-       (compose_raw_closing r1
-          (rhs_raw_closing
-             (transpose_level_raw_closing l2 r2)))).
-Proof.
-  cbn; rewrite rhs_push_transpose_level_raw_closing.
-  destruct (transpose_level_raw_closing_push l2 r2);
-    try rewrite
-      transpose_level_push_normalized_raw_closing_exchange0;
-    easy.
-Qed.
-
-Lemma transpose_level_push_compose_close0 l n r1 r2 :
-  transpose_level_raw_closing_push (S l)
-    (compose_raw_closing (raw_closing_close0 r1 n) r2)
-  = shift_push (transpose_name_raw_closing_push n r2)
-      (transpose_level_raw_closing_push l
-        (compose_raw_closing r1
-           (rhs_raw_closing
-              (transpose_name_raw_closing n r2)))).
-Proof.
-  cbn; rewrite rhs_push_transpose_name_raw_closing.
-  destruct (transpose_name_raw_closing_push n r2);
-    try rewrite
-      transpose_level_push_normalized_raw_closing_exchange0;
-    easy.
-Qed.
-
-Lemma shift_push_weak op :
-  shift_push op weak_op = weak_op.
-Proof. destruct op; easy. Qed.
-
-Definition unshift_push_level op l :=
-  match op with
-  | weak_op => l
-  | cycle_in_op l' => unshift_level l' l
-  | close_op _ => l
-  end.
-
-Definition unshift_push_name op n :=
-  match op with
-  | weak_op => n
-  | cycle_in_op _ => n
-  | close_op n' => unshift_name n' n
-  end.
-
-Lemma shift_level_succ l1 l2 :
-  shift_level (S l1) (S l2)
-  = S (shift_level l1 l2).
-Proof. case_levels l1 l2. Qed.
-
-Lemma foz r l :
-  rhs_raw_closing (closing_rhs_exchange0 r l)
-  = normalized_raw_closing_exchange0
-      (rhs_raw_closing r)
-      (unshift_push_level (rhs_push r) l).
-Proof. destruct r as [? []]; easy. Qed.
-
-Lemma foz2 r n :
-  rhs_raw_closing (closing_rhs_close0 r n)
-  = raw_closing_close0
-      (rhs_raw_closing r)
-      (unshift_push_name (rhs_push r) n).
-Proof. destruct r as [? []]; easy. Qed.
-
-Lemma foo_exchange l1 l2 r :
-  shift_push (transpose_level_raw_closing_push l1 r)
-    (transpose_level_raw_closing_push l2
-       (rhs_raw_closing
-          (transpose_level_raw_closing l1 r))) =
-  transpose_level_raw_closing_push (shift_level l1 l2) r.
-Proof.
-  generalize dependent l1.
-  generalize dependent l2.
-  induction r; intros l2 l1; cbn; try easy.
-  - destruct l1; cbn; try easy.
-    destruct l2; cbn;
-      try rewrite shift_push_weak; try easy.
-    rewrite IHr, shift_level_succ; easy.
-  - destruct l1; cbn; try easy.
-    rewrite foz,
-      rhs_push_transpose_level_raw_closing,
-      transpose_level_push_normalized_raw_closing_exchange0; cbn.
-    destruct l2; cbn.
-    + destruct (transpose_level_raw_closing_push l1 r);
-        cbn; try easy.
-      rewrite transpose_cycle_ins_squared_right; easy.
-    + rewrite shift_level_succ.
-      rewrite <- IHr.
-      destruct (transpose_level_raw_closing_push l1 r),
-        (transpose_level_raw_closing_push l2
-          (rhs_raw_closing
-             (transpose_level_raw_closing l1 r))); try easy; cbn.
-      rewrite transpose_cycle_ins_reverse_right; easy.
-  - destruct l1; cbn; try easy.
-    rewrite foz2, rhs_push_transpose_level_raw_closing; cbn.
-    destruct l2; cbn.
-    + destruct (transpose_level_raw_closing_push l1 r);
-        cbn; try easy.
-      rewrite transpose_closes_squared_right; easy.
-    + rewrite shift_level_succ.
-      rewrite <- IHr.
-      destruct (transpose_level_raw_closing_push l1 r),
-        (transpose_level_raw_closing_push l2
-          (rhs_raw_closing
-             (transpose_level_raw_closing l1 r))); try easy; cbn.
-      rewrite transpose_closes_reverse_right; easy.
-Qed.
-
-Lemma foo_close l n r :
-  shift_push (transpose_level_raw_closing_push l r)
-    (transpose_name_raw_closing_push n
-       (rhs_raw_closing
-          (transpose_level_raw_closing l r))) =
-  transpose_name_raw_closing_push n r.
-Proof.
-  generalize dependent l.
-  generalize dependent n.
-  induction r; intros n' l'; cbn; try easy.
-  - destruct l'; cbn; easy.
-  - destruct l'; cbn; try easy.
-    rewrite foz,
-      rhs_push_transpose_level_raw_closing,
-      transpose_name_push_normalized_raw_closing_exchange0;
-      cbn.
-    rewrite <- IHr with (l := l').
-    destruct (transpose_level_raw_closing_push l' r),
-      (transpose_name_raw_closing_push n'
-         (rhs_raw_closing
-            (transpose_level_raw_closing l' r))); cbn; try easy.
-    rewrite transpose_cycle_ins_reverse_right.
-    easy.
-  - destruct l'; cbn; try easy.
-    rewrite foz2, rhs_push_transpose_level_raw_closing; cbn.
-    rewrite <- IHr with (l := l').
-    destruct (transpose_level_raw_closing_push l' r),
-      (transpose_name_raw_closing_push n'
-         (rhs_raw_closing
-            (transpose_level_raw_closing l' r))); cbn; try easy.
-    rewrite transpose_closes_reverse_right.
-    easy.
-Qed.
-
-Lemma foo l r op :
-  shift_push (transpose_level_raw_closing_push l r)
-    (transpose_push_raw_closing_push op
-       (rhs_raw_closing (transpose_level_raw_closing l r))) =
-  transpose_push_raw_closing_push (shift_level_push l op) r.
-Proof.
-  destruct op; cbn.
-  - rewrite shift_push_weak; easy.
-  - apply foo_exchange.
-  - apply foo_close.
-Qed.
-
-Lemma foo2_exchange n l r :
-  shift_push (transpose_name_raw_closing_push n r)
-      (transpose_level_raw_closing_push l
-         (rhs_raw_closing
-            (transpose_name_raw_closing n r))) =
-    transpose_level_raw_closing_push l r.
-Proof.
-  generalize dependent l.
-  induction r; intros l'; cbn; try easy.
-  - destruct l'; try rewrite shift_push_weak; easy.
-  - rewrite foz,
-      rhs_push_transpose_name_raw_closing,
-      transpose_level_push_normalized_raw_closing_exchange0;
-      cbn.
-    destruct l'.
-    + destruct (transpose_name_raw_closing_push n r);
-        cbn; try easy.
-      rewrite transpose_cycle_ins_squared_right; easy.
-    + rewrite <- IHr.
-      destruct (transpose_name_raw_closing_push n r),
-        (transpose_level_raw_closing_push l'
-          (rhs_raw_closing (transpose_name_raw_closing n r)));
-        cbn; try easy.
-      rewrite transpose_cycle_ins_reverse_right; easy.
-  - rewrite foz2, rhs_push_transpose_name_raw_closing; cbn.
-    destruct l'.
-    + destruct (transpose_name_raw_closing_push n r);
-        cbn; try easy.
-      rewrite transpose_closes_squared_right; easy.
-    + rewrite <- IHr.
-      destruct (transpose_name_raw_closing_push n r),
-        (transpose_level_raw_closing_push l'
-          (rhs_raw_closing (transpose_name_raw_closing n r)));
-        cbn; try easy.
-      rewrite transpose_closes_reverse_right; easy.
-Qed.
-
-Lemma foo2 n r op :
-  shift_push (transpose_name_raw_closing_push n r)
-    (transpose_push_raw_closing_push op
-       (rhs_raw_closing
-          (transpose_name_raw_closing n r))) =
-  transpose_push_raw_closing_push (shift_name_push n op) r.
-Proof.
-  destruct op; cbn.
-  - rewrite shift_push_weak; easy.
-  - 
-
-Lemma transpose_level_compose_raw_closing_push r1 r2 l :
-  transpose_level_raw_closing_push
-    l (compose_raw_closing r1 r2)
+Lemma transpose_push_raw_closing_reverse_middle vo1 vo2 r :
+  unshift_var_opt
+    (transpose_push_raw_closing_push
+       vo1 (transpose_push_raw_closing_raw_closing vo2 r))
+    (transpose_push_raw_closing_push vo2 r)
   = transpose_push_raw_closing_push
-      (transpose_level_raw_closing_push l r1) r2.
+      (unshift_var_opt vo1 vo2)
+      (transpose_push_raw_closing_raw_closing
+         (shift_var_opt vo2 vo1) r).
 Proof.
-  generalize dependent l.
-  generalize dependent r2.
-  induction r1; intros r2 l'; try easy.
-  - destruct l'; cbn; try easy.
-  - destruct l'.
-    + cbn; rewrite rhs_push_transpose_level_raw_closing; cbn.
-      destruct (transpose_level_raw_closing_push l r2);
-        try rewrite
-          transpose_level_push_normalized_raw_closing_exchange0;
-        easy.
-    + rewrite transpose_level_push_compose_exchange0, IHr1; cbn.
-      apply foo.
-  - destruct l'.
-    + cbn; rewrite rhs_push_transpose_name_raw_closing; cbn.
-      destruct (transpose_name_raw_closing_push n r2);
-        try rewrite
-          transpose_level_push_normalized_raw_closing_exchange0;
-        easy.
-    + rewrite transpose_level_push_compose_close0, IHr1; cbn.
-      apply foo.
-
-Lemma transpose_level_compose_raw_closing r1 r2 l :
-  transpose_level_raw_closing l (compose_raw_closing r1 r2)
-  = compose_closing_rhs_raw_closing
-      (transpose_level_raw_closing l r1) r2.
-Proof.
-  generalize dependent O.
-  induction r1; intros O r2; cbn; try easy.
-  - exfalso; apply (level_zero_empty l).
-  - unfold level_sdec; destruct (level_dec l_0 l) as [|neq];
-      subst; cbn; try easy.
-    inversion_level (unshift_level_neq l_0 l (squash neq)).
-    rewrite IHr1.
-    admit.
-  - destruct (transpose_level_closing r2 l0) eqn:Heqrl; cbn.
-    + unfold level_sdec; destruct (level_dec l_0 l) as [|neq];
-        subst; cbn; try solve [rewrite Heqrl; easy].
-      inversion_level (unshift_level_neq l_0 l (squash neq)).
-      rewrite IHr1.
-      admit.
-    + unfold level_sdec; destruct (level_dec l_0 l) as [|neq];
-        subst; cbn; try solve [rewrite Heqrl; easy].
-      inversion_level (unshift_level_neq l_0 l (squash neq)).
-      rewrite IHr1.
-      admit.
-    + unfold level_sdec; destruct (level_dec l_0 l) as [|neq];
-        subst; cbn; try solve [rewrite Heqrl; easy].
-      inversion_level (unshift_level_neq l_0 l (squash neq)).
-      rewrite IHr1.
-      admit.
-  - destruct (transpose_name_closing r2 n) eqn:Heqrn; cbn.
-    + exfalso. admit.
-    + exfalso. admit.
-    + unfold level_sdec; destruct (level_dec l_0 l) as [|neq];
-        subst; cbn; try solve [rewrite Heqrn; easy].
-      inversion_level (unshift_level_neq l_0 l (squash neq)).
-      rewrite IHr1.
-      admit.
+  generalize dependent vo1.
+  generalize dependent vo2.
+  induction r as [|vo3 r]; intros vo2 vo1; cbn; try easy.
+  case_var_zero vo2.
+  - rewrite transpose_push_normalized_raw_closing_push0_push; cbn.
+    rewrite transpose_push_push_zero_left; cbn.
+    rewrite transpose_push_reducing_push_pop; easy.
+  - rewrite transpose_push_normalized_raw_closing_push0_push; cbn.
+    case_var_zero vo1.
+    + rewrite transpose_pushes_squared_left.
+      destruct vo2; easy.
+    + rewrite transpose_push_normalized_raw_closing_push0_push;
+        cbn; reduce_var_zero.
+      rewrite transpose_pushes_reverse_middle.
+      rewrite IHr.
+      rewrite transpose_push_push_pop_zero_reverse_middle.
+      rewrite transpose_push_raw_closing_reverse_right.
+      rewrite transpose_push_push_pop_zero_reverse_right
+        by easy.
+      easy.
 Qed.
 
-Lemma closing_associative {N M O L}
-      (r1 : closing N M) (r2 : closing M O) (r3 : closing O L) :
+Lemma transpose_push_raw_closing_reverse_left vo1 vo2 r :
+  transpose_push_raw_closing_raw_closing vo1
+    (transpose_push_raw_closing_raw_closing vo2 r)
+  = transpose_push_raw_closing_raw_closing
+      (unshift_var_opt vo1 vo2)
+      (transpose_push_raw_closing_raw_closing
+         (shift_var_opt vo2 vo1) r).
+Proof.
+  generalize dependent vo1.
+  generalize dependent vo2.
+  induction r as [|vo3 r]; intros vo2 vo1; cbn; try easy.
+  case_var_zero vo2.
+  - rewrite
+      transpose_push_normalized_raw_closing_push0_raw_closing;
+      cbn.
+    rewrite transpose_push_push_zero_left; cbn.
+    rewrite transpose_push_reducing_push_pop; easy.
+  - rewrite
+      transpose_push_normalized_raw_closing_push0_raw_closing;
+      cbn.
+    case_var_zero vo1.
+    + destruct vo2; easy.
+    + rewrite
+        transpose_push_normalized_raw_closing_push0_raw_closing;
+        cbn; reduce_var_zero.
+      rewrite <- transpose_pushes_reverse_left.
+      rewrite transpose_push_raw_closing_reverse_right.
+      rewrite transpose_push_raw_closing_reverse_middle.
+      rewrite IHr.
+      rewrite transpose_push_push_pop_zero_reverse_middle.
+      rewrite transpose_push_push_pop_zero_reverse_right
+        by easy.
+      easy.
+Qed.
+
+Lemma transpose_push_compose_raw_closing_push r1 r2 vo :
+  transpose_push_raw_closing_push
+    vo (compose_raw_closing r1 r2)
+  = transpose_push_raw_closing_push
+      (transpose_push_raw_closing_push vo r1) r2.
+Proof.
+  generalize dependent vo.
+  generalize dependent r2.
+  induction r1 as [|vo' r1]; intros r2 vo; cbn; try easy.
+  rewrite rhs_push_transpose_push_raw_closing,
+    rhs_raw_closing_transpose_push_raw_closing.
+  rewrite transpose_push_normalized_raw_closing_push0_push; cbn.
+  case_var_zero vo; try easy.
+  rewrite IHr1.
+  apply transpose_push_raw_closing_reverse_right.
+Qed.
+
+Lemma transpose_push_compose_raw_closing_raw_closing r1 r2 vo :
+  normalized_raw_closing r2 ->
+  transpose_push_raw_closing_raw_closing
+    vo (compose_raw_closing r1 r2)
+  = compose_raw_closing
+      (transpose_push_raw_closing_raw_closing vo r1)
+      (transpose_push_raw_closing_raw_closing
+         (transpose_push_raw_closing_push vo r1) r2).
+Proof.
+  generalize dependent vo.
+  generalize dependent r2.
+  induction r1 as [|vo' r1]; intros r2 vo Hnorm; cbn; try easy.
+  rewrite rhs_push_transpose_push_raw_closing,
+    rhs_raw_closing_transpose_push_raw_closing.
+  rewrite
+    transpose_push_normalized_raw_closing_push0_raw_closing;
+    cbn.
+  case_var_zero vo; try easy.
+  rewrite IHr1;
+    try (apply transpose_push_raw_closing_raw_closing_normalized;
+         easy).
+  rewrite transpose_push_raw_closing_reverse_left.
+  rewrite transpose_push_compose_raw_closing_push.
+  rewrite transpose_push_raw_closing_reverse_middle.
+  rewrite compose_normalized_raw_closing_push0;
+    try (apply transpose_push_raw_closing_raw_closing_normalized;
+         easy); cbn.
+  rewrite rhs_push_transpose_push_raw_closing,
+    rhs_raw_closing_transpose_push_raw_closing.
+  easy.
+Qed.
+
+Lemma raw_closing_associative r1 r2 r3 :
+  normalized_raw_closing r3 ->
+  compose_raw_closing r1 (compose_raw_closing r2 r3)
+  = compose_raw_closing (compose_raw_closing r1 r2) r3.
+Proof.
+  generalize dependent r2.
+  generalize dependent r3.
+  induction r1; cbn; intros r3 r2 Hnorm; try easy.
+  rewrite compose_normalized_raw_closing_push0 by easy; cbn.
+  rewrite !rhs_push_transpose_push_raw_closing,
+    !rhs_raw_closing_transpose_push_raw_closing.
+  rewrite transpose_push_compose_raw_closing_raw_closing
+    by easy.
+  rewrite IHr1
+    by (apply transpose_push_raw_closing_raw_closing_normalized;
+        easy).
+  rewrite transpose_push_compose_raw_closing_push.
+  easy.
+Qed.
+
+Lemma closing_associative r1 r2 r3 :
   compose_closing r1 (compose_closing r2 r3)
   = compose_closing (compose_closing r1 r2) r3.
 Proof.
-  induction r1; cbn; try easy.
-  - rewrite IHr1; easy.
-  - 
-
-Inductive closing : nat -> nat -> Set :=
-| closing_nil : closing 0 0
-| closing_weak0 : forall N M,
-  closing N M -> closing (S N) M
-| closing_exchange0 : forall N M,
-    closing N M -> level (S M) -> closing (S N) (S M)
-| closing_close0 : forall N M,
-    closing N M -> name -> closing (S N) M.
+  destruct r1, r2, r3.
+  apply lift_closing_eq; cbn.
+  apply raw_closing_associative; easy.
+Qed.
